\begin{answer}
Using Bayes rule.

\begin{align*}
    & p(t^{(i)}=1\mid y^{(i)} = 1, x^{(i)}) = \frac{p(y^{(i)} = 1\mid t^{(i)}=1, x^{(i)})p(t^{(i)}=1\mid x^{(i)})}{p(y^{(i)}=1\mid x^{(i)})} \\
\end{align*}

And we know that,
\begin{align*}
    & p(y^{(i)}=1, t^{(i)}=1\mid x^{(i)}) = p(y^{(i)}=1\mid t^{(i)}=1, x^{(i)}) p(t^{(i)}=1\mid x^{(i)}) = \alpha \cdot p(t^{(i)}=1\mid x^{(i)})\\
    & p(y^{(i)}=1, t^{(i)}=0\mid x^{(i)}) = p(y^{(i)}=1\mid t^{(i)}=0, x^{(i)}) p(t^{(i)}=0\mid x^{(i)}) = 0 \cdot p(t^{(i)}=1\mid x^{(i)}) = 0\\
    &\begin{aligned}
    p(y^{(i)}=1\mid x^{(i)}) &= \sum_t p(y^{(i)}=1, t^{(i)}=t\mid x^{(i)}) \\
    &= p(y^{(i)}=1, t^{(i)}=1\mid x^{(i)}) + p(y^{(i)}=1, t^{(i)}=0\mid x^{(i)}) \\
    &= \alpha \cdot p(t^{(i)}=1\mid x^{(i)})\\
    \end{aligned}
\end{align*}

Therefore,

\begin{align*}
    p(t^{(i)}=1\mid y^{(i)} = 1, x^{(i)}) &= \frac{p(y^{(i)} = 1\mid t^{(i)}=1, x^{(i)})p(t^{(i)}=1\mid x^{(i)})}{p(y^{(i)}=1\mid x^{(i)})} \\
    &= \frac{\alpha \cdot p(t^{(i)}=1\mid x^{(i)})}{\alpha \cdot p(t^{(i)}=1\mid x^{(i)})} = 1\\
\end{align*}
\end{answer}
