\begin{answer}
Hessian matrix is defined as,

$$
\begin{aligned}
H(f) &= 
\begin{bmatrix} 
    {\partial^2 f \over {\partial x_1}^2} & {\partial^2 f \over {\partial x_1\partial x_2}} & \cdots & {\partial^2 f \over {\partial x_1\partial x_n}}\\
    {\partial^2 f \over {\partial x_2 \partial x_1}} & \ddots & & \vdots \\
    \vdots & & \ddots & \vdots\\
    {\partial^2 f \over {\partial x_n \partial x_1}} & \cdots & & {\partial^2 f \over {\partial x_n}^2}
\end{bmatrix} \\
H(J) &=
\begin{bmatrix} 
    {\partial^2 J \over {\partial \theta_1}^2} &  {\partial^2 J \over {\partial \theta_1\partial \theta_2}}\\
    {\partial^2 J \over {\partial \theta_2 \partial \theta_1}} & {\partial^2 J \over {\partial \theta_2}^2} \\
\end{bmatrix}
\end{aligned}
$$

$$
\begin{aligned}
{\partial J \over {\partial \theta_1}} 
&= {\partial \over {\partial \theta_1}} \left( 
- {1 \over n} \sum_{i=1}^n \left( y^{(i)}\log({1 \over {1 + e^{-(\theta_1 x_1^{(i)} + \theta_2 x_2^{(i)})}}}) 
+ (1-y^{(i)}) \log({e^{-(\theta_1 x_1^{(i)} + \theta_2 x_2^{(i)})} \over {1 + e^{-(\theta_1 x_1^{(i)} + \theta_2 x_2^{(i)})}}})\right) \right) \\
&=  - {1 \over n} \sum_{i=1}^n \left( 
y^{(i)} {x_1^{(i)} e^{-(\theta_1 x_1^{(i)} + \theta_2 x_2^{(i)})} \over {1 + e^{-(\theta_1 x_1^{(i)} + \theta_2 x_2^{(i)})}}} 
- (1-y^{(i)}) {x_1^{(i)} e^{(\theta_1 x_1^{(i)} + \theta_2 x_2^{(i)})} \over {1 + e^{(\theta_1 x_1^{(i)} + \theta_2 x_2^{(i)})}}}
\right) \\
&=  - {1 \over n} \sum_{i=1}^n \left( 
y^{(i)} {x_1^{(i)} \over {1 + e^{\theta^T x^{(i)}}}} 
- (1-y^{(i)}) {x_1^{(i)} \over {1 + e^{-\theta^T x^{(i)}}}}
\right) \\
{\partial J \over {\partial \theta_2}} 
&= - {1 \over n} \sum_{i=1}^n \left( 
y^{(i)} {x_2^{(i)} \over {1 + e^{\theta^T x^{(i)}}}} 
- (1-y^{(i)}) {x_2^{(i)} \over {1 + e^{-\theta^T x^{(i)}}}}
\right) \\
\end{aligned}
$$

Let $\sigma := 1/(1 + e^{-\theta^T x^{(i)}})$ then the equations are simplified as,

$$
\begin{aligned}
{\partial J \over {\partial \theta_1}} 
&= - {1 \over n} \sum_{i=1}^n \left( 
y^{(i)} x_1^{(i)} (1 - \sigma)
- (1-y^{(i)}) x_1^{(i)} \sigma
\right) 
= - {1 \over n} \sum_{i=1}^n x_1^{(i)} \left(
y^{(i)} - \sigma
\right) \\
{\partial J \over {\partial \theta_2}} 
&= - {1 \over n} \sum_{i=1}^n \left( 
y^{(i)} x_2^{(i)} (1 - \sigma)
- (1-y^{(i)}) x_2^{(i)} \sigma
\right) 
= - {1 \over n} \sum_{i=1}^n x_2^{(i)} \left(
y^{(i)} - \sigma
\right) \\
{\partial^2 J \over {\partial \theta_1}^2} 
&= {1 \over n} \sum_{i=1}^n \left( 
(x_1^{(i)})^2 \sigma (1-\sigma)
\right) \\
{\partial^2 J \over {\partial \theta_1\partial \theta_2}} 
&= {1 \over n} \sum_{i=1}^n \left( 
(x_1^{(i)}x_2^{(i)}) \sigma (1-\sigma)
\right) \\
{\partial^2 J \over {\partial \theta_2 \partial \theta_1}} 
&= {1 \over n} \sum_{i=1}^n \left( 
(x_1^{(i)}x_2^{(i)}) \sigma (1-\sigma)
\right) \\
{\partial^2 J \over {\partial \theta_2}^2}
&= {1 \over n} \sum_{i=1}^n \left( 
(x_2^{(i)})^2 \sigma (1-\sigma)
\right) \\
\end{aligned}
$$

Finally, the Hessian matrix $H$ represents as,

$$
H = {1 \over n}
\begin{bmatrix}
    \sum_{i=1}^n \sigma (1-\sigma) ((x_1^{(i)})^2) & \sum_{i=1}^n \sigma (1-\sigma) (x_1^{(i)}x_2^{(i)}) \\
    \sum_{i=1}^n \sigma (1-\sigma) (x_1^{(i)}x_2^{(i)}) & \sum_{i=1}^n \sigma (1-\sigma) ((x_2^{(i)})^2) \\
\end{bmatrix}.
$$

Now, prove $z^T H z \geq 0$.

$$
\begin{aligned}
z^T H z &=
\begin{bmatrix}
    z_1 & z_2 \\
\end{bmatrix}
H
\begin{bmatrix}
    z_1 \\
    z_2 \\
\end{bmatrix} \\
&= {1 \over n} 
\begin{bmatrix}
    z_1 & z_2 \\
\end{bmatrix}
\begin{bmatrix}
    \sum_{i=1}^n \sigma (1-\sigma) z_1 (x_1^{(i)})^2 + z_2 (x_1^{(i)}x_2^{(i)}) \\
    \sum_{i=1}^n \sigma (1-\sigma) z_1 (x_1^{(i)}x_2^{(i)}) + z_2 (x_2^{(i)})^2 \\
\end{bmatrix} \\
&= {1 \over n}
\sum_{i=1}^n \sigma (1-\sigma) \left( z_1^2 (x_1^{(i)})^2 + 2 z_1 z_2 (x_1^{(i)}x_2^{(i)}) + z_2^2 (x_2^{(i)})^2 \right) \\
&= {1 \over n} \sum_{i=1}^n \sigma (1-\sigma) \left( z_1 x_1^{(i)}+ z_2 x_2^{(i)} \right)^2 \geq 0.
\end{aligned}
$$
\end{answer}
