\begin{answer}

\begin{align*}
    \mathbb{E}[Y;\eta] &= \int y\,p(y;\eta)\,dy \\
    \frac{\partial}{\partial\eta}\int p(y;\eta)\,dy &= \int \frac{\partial}{\partial\eta} p(y;\eta)\,dy \\
    &= \int b(y)\exp(\eta\,y - a(\eta))\cdot \left(y - \frac{\partial}{\partial\eta}a(\eta)\right)\,dy
\end{align*}

Note that

\begin{align*}
    &\int p(y;\eta)\,dy = 1 \\
    &\frac{\partial}{\partial\eta}\int p(y;\eta)\,dy = 0 \\
    &\int b(y)\exp(\eta\,y - a(\eta))\cdot \left(y - \frac{\partial}{\partial\eta}a(\eta)\right)\,dy = 0
\end{align*}

Therefore

\begin{align*}
    \mathbb{E}[Y;\eta] &= \int y\,p(y;\eta)\,dy \\
    &= \int y\,b(y)\exp(\eta\,y - a(\eta))\,dy \\
    &= \int b(y)\exp(\eta\,y - a(\eta))\cdot \frac{\partial}{\partial\eta}a(\eta)\,dy \\
    &= \frac{\partial}{\partial\eta}a(\eta) \int b(y)\exp(\eta\,y - a(\eta))\,dy \\
    &= \frac{\partial}{\partial\eta}a(\eta) \int p(y;\eta)\,dy \\
    &= \frac{\partial}{\partial\eta}a(\eta)
\end{align*}

\end{answer}
