\begin{answer}
\begin{align*}
    \frac{\partial}{\partial\eta}\left(\frac{\partial}{\partial\eta}a(\eta)\right) &= \frac{\partial}{\partial\eta} \mathbb{E}[Y;\eta] \\
    &= \frac{\partial}{\partial\eta} \int y\,b(y)\exp(\eta\,y - a(\eta))\,dy \\
    &= \int y\,b(y)\exp(\eta\,y - a(\eta))\cdot \left(y - \frac{\partial}{\partial\eta}a(\eta)\right)\,dy \\
    &= \int y^2\,b(y)\exp(\eta\,y - a(\eta))\,dy - \frac{\partial}{\partial\eta}a(\eta)\int y\,b(y)\exp(\eta\,y - a(\eta))\,dy \\
    &= \mathbb{E}[Y^2;\eta] - \mathbb{E}[Y;\eta]\cdot\mathbb{E}[Y;\eta] \\
    &= \textrm{Var}[Y;\eta]
\end{align*}
\end{answer}
